Updating trace equivalence

theories/MP/GLTraceEquiv.v
@@ -21,11 +21,99 @@ Section TraceEquiv.
   Definition trace_equiv G P :=
     forall a, exists G' P', g_lts a G G' <-> l_lts a P P'.
 
+  Fixpoint add_head p (Q : MsgQ) :=
+    match Q with
+    | [::] => [:: (p.1, [:: p.2])]
+    | h :: t => if h.1 == p.1 then (h.1, p.2 :: h.2) :: t
+                else h :: add_head p t
+    end.
+
+  Notation msg m := (m.1, inr m.2).
+  Notation lab m l := (m.1, inl l).
+
+  Fixpoint q_proj G (p : role) : option (MsgQ * l_ty):=
+    match G with
+    | rg_end => Some ([::], l_end)
+    | rg_msg m G =>
+      match q_proj G p with
+      | Some QP => if m.snd == m.rcv then None
+                   else if m.snd == p
+                        then Some (QP.1, l_send m.rcv m.typ QP.2)
+                        else if m.rcv == p
+                             then Some (QP.1, l_recv m.snd m.typ QP.2)
+                             else Some QP
+      | None => None
+      end
+    | rg_rcv m G =>
+      match q_proj G p with
+      | Some QP => if m.snd == m.rcv then None
+                   else if m.snd == p
+                        then Some (add_head (msg m) QP.1, QP.2)
+                        else if m.rcv == p
+                             then Some (QP.1, l_recv m.snd m.typ QP.2)
+                             else Some QP
+      | None => None
+      end
+        (* )
+    | rg_brn m K =>
+      let KL := map (fun X => (X.1, q_proj X.2 r)) K in
+    if m.snd == m.rcv
+    then None
+    else if m.snd == p
+         then ml_sel q K
+         else if q == r
+              then ml_brn p K
+              else merge_all K.
+
+      match q_proj G p with
+      | Some QP => if m.snd == m.rcv then None
+                   else if m.snd == p
+                        then Some (add_head (msg m) QP.1, QP.2)
+                        else if m.rcv == p
+                             then Some (QP.1, l_recv m.snd m.typ QP.2)
+                             else Some QP
+      | None => None
+      end
+    | g_brn p K =>
+      let KL := map (fun X => (X.1, project X.2 r)) K in
+      project_brn p r KL *)
+    | _ => None
+    end.
+
+  Definition project_brn (p : g_prefix) (r : role) (K : seq (lbl * option l_ty)) :=
+    let: ((p, q), t) := p in
+    if p == q
+    then None
+    else if p == r
+         then ml_sel q K
+         else if q == r
+              then ml_brn p K
+              else merge_all K.
+
+  Definition q_union (Q1 Q2 : MsgQ) := Q1 ++ Q2.
+
+  Fixpoint q_project G ps :=
+    match ps with
+    | [::] => Some ([::], [::])
+    | h :: t => match q_proj G h , q_project G t with
+                | Some (Q', L), Some (Q, P) => Some (q_union Q Q', (h, L) :: P)
+                | _, _ => None
+                end
+    end.
+
+  Definition q_projection G :=
+    q_project G (rg_parts G).
+
+  Lemma g_trequiv G :
+    forall P,
+    q_projection G == Some P ->
+    trace_equiv G P.
+  Admitted.
+
   Theorem global_local_trequiv G :
     forall P,
     projection G == Some P ->
     trace_equiv (init G) ([::], P).
-  Proof.
   Admitted.
 
 End TraceEquiv.
